verified/Seq.dfy
@@ -1,0 +1,16 @@
+//-----------------------------------------------------------------------------
+// Sequence Utilities
+//-----------------------------------------------------------------------------
+
+function SeqLength<T>(s:seq<T>) : int { |s| }
+function SeqDrop<T>(s:seq<T>, tail:int) : seq<T> 
+    requires 0 <= tail <= |s|;                                           
+    { s[..tail] }
+function SeqAppendElt<T>(s:seq<T>, elt:T) : seq<T> { s + [elt] }
+function SeqBuild<T>(elt:T) : seq<T> { [elt] }
+function SeqRepeat<T>(count:nat, elt:T) : seq<T>
+    ensures |SeqRepeat<T>(count, elt)| == count
+    ensures forall e :: e in SeqRepeat<T>(count, elt) ==> e == elt
+{
+    if count == 0 then [] else [elt] + SeqRepeat<T>(count - 1, elt)
+}
